Ordered supports
Signed-off-by: zeramorphic <zeramorphic@proton.me>

ConNF/Counting/OrdSupport.lean
@@ -15,6 +15,8 @@ variable [Params.{u}] {α : Λ} [BasePositions] [FoaAssumptions α] {β : Iic α
 structure OrdSupport (β : Iic α) where
   /-- The set of support conditions in this ordered support. -/
   carrier : Set (SupportCondition β)
+  /-- The carrier set is small. -/
+  carrier_small : Small carrier
   /-- An order on `carrier`. -/
   r : carrier → carrier → Prop
   /-- `r` is a well order. -/
@@ -33,16 +35,152 @@ instance : Membership (SupportCondition β) (OrdSupport β) where
 instance : CoeSort (OrdSupport β) (Type _) :=
   ⟨fun S => { x : SupportCondition β // x ∈ S }⟩
 
+instance : HasSubset (OrdSupport β) where
+  Subset S T := ∀ ⦃c : SupportCondition β⦄, c ∈ S → c ∈ T
+
 @[simp, norm_cast]
 theorem coe_sort_coe (S : OrdSupport β) : ((S : Set (SupportCondition β)) : Type _) = S :=
   rfl
 
-instance : IsWellOrder S S.r := S.r_isWellOrder
+theorem small (S : OrdSupport β) : Small (S : Set (SupportCondition β)) :=
+  S.carrier_small
+
+instance isWellOrder (S : OrdSupport β) : IsWellOrder S S.r := S.r_isWellOrder
 
 instance : PartialOrder S := partialOrderOfSO S.r
 
 open scoped Classical in
 noncomputable instance : LinearOrder S := linearOrderOfSTO S.r
+
+@[ext]
+theorem ext {S T : OrdSupport β} (h₁ : S ⊆ T) (h₂ : T ⊆ S)
+    (h : ∀ c d : S, c < d ↔ (⟨c, h₁ c.prop⟩ : T) < ⟨d, h₁ d.prop⟩) :
+    S = T := by
+  obtain ⟨S, _, r, _⟩ := S
+  obtain ⟨T, _, s, _⟩ := T
+  cases subset_antisymm (show (S : Set (SupportCondition β)) ⊆ T from h₁) h₂
+  simp only [mk.injEq, heq_eq_eq, true_and]
+  ext c d
+  exact h c d
+
+instance : SMul (Allowable β) (OrdSupport β) where
+  smul ρ S := {
+    carrier := {c | ρ⁻¹ • c ∈ S}
+    carrier_small := Small.preimage (MulAction.injective ρ⁻¹) S.small
+    r := fun c d => (⟨ρ⁻¹ • c.val, c.prop⟩ : S) < ⟨ρ⁻¹ • d.val, d.prop⟩
+    r_isWellOrder := by
+      refine isWellOrder_invImage S.isWellOrder
+        (fun c : {c // ρ⁻¹ • c ∈ S} => ⟨ρ⁻¹ • c.val, c.prop⟩) ?_
+      intros c d h
+      simp only [Subtype.mk.injEq, smul_left_cancel_iff, Subtype.coe_injective.eq_iff] at h
+      exact h
+  }
+
+@[simp]
+theorem smul_mem {ρ : Allowable β} {S : OrdSupport β} {c : SupportCondition β} :
+    c ∈ ρ • S ↔ ρ⁻¹ • c ∈ S :=
+  Iff.rfl
+
+theorem inv_smul_mem {ρ : Allowable β} {S : OrdSupport β} {c : SupportCondition β} :
+    ρ⁻¹ • c ∈ S ↔ c ∈ ρ • S :=
+  smul_mem.symm
+
+theorem smul_mem_smul {ρ : Allowable β} {S : OrdSupport β} {c : SupportCondition β} :
+    ρ • c ∈ ρ • S ↔ c ∈ S := by
+  simp only [smul_mem, inv_smul_smul]
+
+theorem smul_mem_inv {ρ : Allowable β} {S : OrdSupport β} {c : SupportCondition β} :
+    c ∈ ρ⁻¹ • S ↔ ρ • c ∈ S := by
+  simp only [smul_mem, inv_inv]
+
+@[simp]
+theorem lt_iff_smul {ρ : Allowable β} {S : OrdSupport β} {c d : ρ • S} :
+    c < d ↔ (⟨ρ⁻¹ • c.val, c.prop⟩ : S) < ⟨ρ⁻¹ • d.val, d.prop⟩ :=
+  Iff.rfl
+
+instance : MulAction (Allowable β) (OrdSupport β) where
+  one_smul S := by
+    refine ext ?_ ?_ ?_
+    · intro c hc
+      simp only [smul_mem, inv_one, one_smul] at hc
+      exact hc
+    · intro c hc
+      simp only [smul_mem, inv_one, one_smul]
+      exact hc
+    · intro c d
+      simp only [lt_iff_smul, inv_one, one_smul]
+  mul_smul ρ₁ ρ₂ S := by
+    refine ext ?_ ?_ ?_
+    · intro c hc
+      simp only [smul_mem, mul_inv_rev, mul_smul] at hc
+      exact hc
+    · intro c hc
+      simp only [smul_mem, mul_inv_rev, mul_smul]
+      exact hc
+    · intro c d
+      simp only [lt_iff_smul, mul_inv_rev, mul_smul]
+
+/-- An ordered support is strong if every element of its domain is reduced, every reduced condition
+it constrains lies in its domain, and its order agrees with the constrains relation. -/
+structure Strong (S : OrdSupport β) : Prop where
+  reduced_of_mem (c : S) : Reduced c.val.value
+  transConstrains_mem (c : SupportCondition β) (d : S) : Reduced c.value → c <[α] d → c ∈ S
+  lt_of_transConstrains : (c d : S) → c.val <[α] d.val → c < d
+
+/-- `T` *extends* `S` if it is a well-order that end-extends `S`. -/
+structure Extends (T S : OrdSupport β) : Prop where
+  mem_of_mem (c : S) : c.val ∈ T
+  lt_iff_lt (c d : S) :
+    c < d ↔ (⟨c, mem_of_mem c⟩ : T) < ⟨d, mem_of_mem d⟩
+  /-- If `c` is in `S ∩ T` and `d` is in `T \ S`, then `c` comes before `d`. -/
+  get_lt_get (c : S) (d : T) (hd : d.val ∉ S) :
+    ⟨c, mem_of_mem c⟩ < d
+
+instance : LE (OrdSupport β) where
+  le S T := Extends T S
+
+instance : PartialOrder (OrdSupport β) where
+  le_refl S := by
+    constructor
+    · intro c hc
+      rfl
+    · intro c d hd
+      cases hd d.prop
+  le_trans S T U hST hTU := by
+    constructor
+    · intro c d
+      rw [hST.lt_iff_lt, hTU.lt_iff_lt]
+    · intro c d hdS
+      by_cases hdT : d.val ∈ T
+      · have := hST.get_lt_get c ⟨d, hdT⟩ hdS
+        rw [hTU.lt_iff_lt] at this
+        exact this
+      · have := hTU.get_lt_get ⟨c, hST.mem_of_mem c⟩ d hdT
+        exact this
+  le_antisymm S T hST hTS := by
+    refine ext (fun c hc => hST.mem_of_mem ⟨c, hc⟩) (fun c hc => hTS.mem_of_mem ⟨c, hc⟩) ?_
+    intro c d
+    rw [hST.lt_iff_lt]
+
+theorem smul_le_smul {S T : OrdSupport β} (h : S ≤ T) (ρ : Allowable β) : ρ • S ≤ ρ • T := by
+  constructor
+  · intro c d
+    exact h.lt_iff_lt ⟨ρ⁻¹ • c.val, c.prop⟩ ⟨ρ⁻¹ • d.val, d.prop⟩
+  · intro c d
+    exact h.get_lt_get ⟨ρ⁻¹ • c.val, c.prop⟩ ⟨ρ⁻¹ • d.val, d.prop⟩
+  · intro c
+    exact h.mem_of_mem ⟨ρ⁻¹ • c.val, c.prop⟩
+
+theorem smul_le_iff_le_inv {S T : OrdSupport β} (ρ : Allowable β) : S ≤ ρ⁻¹ • T ↔ ρ • S ≤ T := by
+  constructor
+  · intro h
+    have := smul_le_smul h ρ
+    rw [smul_inv_smul] at this
+    exact this
+  · intro h
+    have := smul_le_smul h ρ⁻¹
+    rw [inv_smul_smul] at this
+    exact this
 
 end OrdSupport
 
